LambdaLetDollar.v
@@ -107,6 +107,13 @@ Definition mapV' {A B} (f : A → B) (v : val' A) : val' B :=
   | val_s_0' => val_s_0'
   end.
 
+Definition mapP' {A B : Type} (f : A -> B) (p : non' A) : non' B :=
+  match p with
+  | non_app' e1 e2 => non_app' (map' f e1) (map' f e2)
+  | non_dol' e1 e2 => non_dol' (map' f e1) (map' f e2)
+  | non_let' e1 e2 => non_let' (map' f e1) (map' (option_map f) e2)
+  end.
+
 Lemma map_val_is_val' : ∀ {A B} (v : val' A) (f : A → B),
   ∃ w, map' f (val_to_tm' v) = val_to_tm' w.
 Proof.
@@ -115,10 +122,25 @@ Proof.
   - exists val_s_0'; reflexivity.
 Qed.
 
+Lemma map_non_is_non' : ∀ {A B} (p1 : non' A) (f : A → B),
+  ∃ p2, map' f (non_to_tm' p1) = non_to_tm' p2.
+Proof.
+  intros. destruct p1; cbn.
+  - eexists (non_app' _ _). reflexivity.
+  - eexists (non_dol' _ _). reflexivity.
+  - eexists (non_let' _ _). reflexivity.
+Qed.
+
 Lemma mapV_is_map' : ∀ {A B} v (f : A → B),
   val_to_tm' (mapV' f v) = map' f (val_to_tm' v).
 Proof.
   intros. destruct v; auto.
+Qed.
+
+Lemma mapP_is_map' : ∀ {A B} p (f : A → B),
+  non_to_tm' (mapP' f p) = map' f (non_to_tm' p).
+Proof.
+  intros. destruct p; auto.
 Qed.
 
 Lemma map_map_law' : forall A e B C (f:A->B) (g:B->C),
@@ -168,6 +190,17 @@ Definition bindV' {A B} (f : A → tm' B) (v : val' A) : val' B :=
       end) e)
   end.
 
+Definition bindP' {A B : Type} (f : A -> tm' B) (p : non' A) : non' B :=
+  match p with
+  | non_app' e1 e2 => non_app' (bind' f e1) (bind' f e2)
+  | non_dol' e1 e2 => non_dol' (bind' f e1) (bind' f e2)
+  | non_let' e1 e2 => non_let' (bind' f e1) (bind' (fun a' => 
+      match a' with
+      | None   => tm_var' None
+      | Some a => map' Some (f a)
+      end) e2)
+  end.
+
 Lemma bind_val_is_val' : ∀ {A B} (v : val' A) (f : A → tm' B),
   ∃ w, bind' f (val_to_tm' v) = val_to_tm' w.
 Proof.
@@ -180,6 +213,12 @@ Lemma bindV_is_bind' : ∀ {A B} v (f : A → tm' B),
   val_to_tm' (bindV' f v) = bind' f (val_to_tm' v).
 Proof.
   intros. destruct v; auto.
+Qed.
+
+Lemma bindP_is_bind' : ∀ {A B} p (f : A → tm' B),
+  non_to_tm' (bindP' f p) = bind' f (non_to_tm' p).
+Proof.
+  intros. destruct p; auto.
 Qed.
 
 Lemma bind_map_law' : ∀ {A B C} (f : B → tm' C) (g : A → B) e,
